src/lowparse/LowParse.Low.List.fst
@@ -12,7 +12,9 @@ module M = LowStar.Modifies
 module I32 = FStar.Int32
 module Cast = FStar.Int.Cast
 
+unfold
 let validate32_list_inv'
+  [| validator32_cls |]
   (#k: parser_kind)
   (#t: Type0)
   (p: parser k t)
@@ -26,7 +28,12 @@ let validate32_list_inv'
 = k.parser_kind_low > 0 /\
   is_slice (G.reveal h0) input len /\
   B.disjoint input read_so_far /\
-  M.modifies (M.loc_buffer read_so_far) (G.reveal h0) h /\
+  M.loc_disjoint (M.loc_buffer read_so_far) validator32_error_loc /\
+  M.loc_disjoint (M.loc_buffer input) validator32_error_loc /\
+//  M.loc_disjoint (M.loc_union (M.loc_buffer read_so_far) (M.loc_buffer input)) validator32_error_loc /\
+  M.modifies (M.loc_union validator32_error_loc (M.loc_buffer read_so_far)) (G.reveal h0) h /\
+  validator32_error_inv (Ghost.reveal h0) /\
+  validator32_error_inv h /\
   is_slice h input len /\
   B.live h read_so_far /\
   (
@@ -34,7 +41,7 @@ let validate32_list_inv'
     let ps0 = parse (parse_list p) (B.as_seq (G.reveal h0) input) in
     if stop
     then
-      validator32_postcond (parse_list p) input len (G.reveal h0) v_read_so_far (G.reveal h0)
+      validator32_postcond'  (parse_list p) input len (G.reveal h0) v_read_so_far (G.reveal h0)
     else
       I32.v v_read_so_far >= 0 /\
       I32.v v_read_so_far <= I32.v len /\ (
@@ -43,7 +50,9 @@ let validate32_list_inv'
       True
         ))
 
+unfold
 let validate32_list_inv
+  [| validator32_cls |]
   (#k: parser_kind)
   (#t: Type0)
   (p: parser k t)
@@ -59,7 +68,36 @@ let validate32_list_inv
 #reset-options "--z3rlimit 64 --z3cliopt smt.arith.nl=false"
 
 inline_for_extraction
+let validate32_list_body_case1
+  [| cls: validator32_cls |]
+  (#k: parser_kind)
+  (#t: Type0)
+  (#p: parser k t)
+  (v: validator32 p)
+  (input: buffer8)
+  (len: I32.t)
+  (read_so_far: pointer I32.t)
+  (h0: G.erased HS.mem)
+  (u: unit)
+: HST.Stack bool
+  (requires (fun h ->
+    validate32_list_inv p input len read_so_far h0 h false /\ (
+    let v_read_so_far = Seq.index (B.as_seq h read_so_far) 0 in
+    v_read_so_far = len
+  )))
+  (ensures (fun h stop h' ->
+    validate32_list_inv p input len read_so_far h0 h false /\
+    validate32_list_inv p input len read_so_far h0 h' stop
+  ))
+= B.upd read_so_far 0ul 0l;
+  let h' = HST.get () in
+  assert (validator32_error_inv h');
+  // assert (validator32_error_inv h' ==> validate32_list_inv p input len read_so_far h0 h' true);
+  true
+
+inline_for_extraction
 let validate32_list_body
+  [| cls: validator32_cls |]
   (#k: parser_kind)
   (#t: Type0)
   (#p: parser k t)
@@ -80,18 +118,17 @@ let validate32_list_body
   let v_read_so_far = B.index read_so_far 0ul in
   if v_read_so_far = len
   then begin
-    B.upd read_so_far 0ul 0l;
-    f ();
-    true
+    validate32_list_body_case1 #cls v input len read_so_far h0 u
   end
   else begin
+    let h1 = HST.get () in
     let res = v (B.offset input (Cast.int32_to_uint32 v_read_so_far)) (len `I32.sub` v_read_so_far) in
  (* now we require that the element parser consumes at least one byte *)
-//    assume (res <> len `I32.sub` v_read_so_far);
     if res `I32.lt` 0l // || res = len `I32.sub` v_read_so_far
     then begin
       B.upd read_so_far 0ul res; // (-1l);
       f ();
+      let h' = HST.get () in
       true
     end else begin
       let read_so_far' = len `I32.sub` res in
@@ -118,15 +155,19 @@ let validate32_list_body
 
 inline_for_extraction
 let validate32_list
+  [| cls: validator32_cls |]
   (#k: parser_kind)
   (#t: Type0)
   (#p: parser k t)
-  (v: validator32 p { k.parser_kind_low > 0 } )
+  (v: validator32 #cls p { k.parser_kind_low > 0 } )
 : Tot (validator32 (parse_list p))
 = fun input len ->
-  HST.push_frame ();  
+  HST.push_frame ();
+  let h_ = HST.get () in
+  assert (validator32_error_inv h_);
   let read_so_far = B.alloca 0l 1ul in
   let h = HST.get () in
+  assert (validator32_error_inv h);
   let h0 = G.hide h in
   C.Loops.do_while
     (validate32_list_inv p input len read_so_far h0)
