src/lowparse/LowParse.Low.Option.fst
@@ -5,7 +5,7 @@ include LowParse.Low.Base
 module I32 = FStar.Int32
 
 inline_for_extraction
-let validate32_option (#k: parser_kind) (#t: Type) (#p: parser k t) (v: validator32 p) : Tot (validator32 (parse_option p)) =
+let validate32_option (#k: parser_kind) (#t: Type) (#p: parser k t) [| validator32_cls |] (v: validator32 p) : Tot (validator32 (parse_option p)) =
   fun input len ->
   let r = v input len in
   if r `I32.lt` 0l
